refactor through add_group, group, add_monoid, monoid

src/model_theory/algebraic.lean
@@ -18,65 +18,188 @@ import model_theory.syntax
 * `first_order.language.Theory.comm_ring` defines the theory of commutative rings.
 * `first_order.language.Theory.field` defines the theory of fields.
 -/
-universes u
+universes u v u' v'
 
 namespace first_order
 namespace language
 open_locale first_order
 open Structure
 
+section sentences
+
+variables {L : language.{u v}} (c₀ c₁ : L.constants) (i : L.functions 1) (a m : L.functions 2)
+
+/-- The sentence indicating that a binary functionol is commutative. -/
+protected def comm : L.sentence := ∀' ∀' (m.apply₂ &0 &1 =' m.apply₂ &1 &0)
+
+/-- The sentence indicating that a binary function symbol is associative. -/
+protected def assoc : L.sentence :=
+∀' ∀' ∀' (m.apply₂ (m.apply₂ &0 &1) &2 =' m.apply₂ &0 (m.apply₂ &1 &2))
+
+/-- The sentence indicating that applying a constant symbol on the left of
+  a binary symbol is the identity. -/
+def id_left : L.sentence :=
+∀' (m.apply₂ c₁.term &0 =' &0)
+
+/-- The sentence indicating that applying a constant symbol on the right of
+  a binary symbol is the identity. -/
+def id_right : L.sentence :=
+∀' (m.apply₂ &0 c₁.term =' &0)
+
+/-- The sentence indicating that left composing a unary symbol with a binary symbol
+  is equal to a constant symbol. -/
+def cancel_left : L.sentence :=
+∀' (m.apply₂ (i.apply₁ &0) &0 =' c₁.term)
+
+/-- The sentence indicating that right composing a unary symbol with a binary symbol
+  is equal to a constant symbol. -/
+def cancel_right : L.sentence :=
+∀' (m.apply₂ &0 (i.apply₁ &0) =' c₁.term)
+
+/-- The sentence indicating that a binary function symbol distributes over another -/
+protected def distrib : L.sentence :=
+∀' ∀' ∀' (m.apply₂ (a.apply₂ &0 &1) &2 =' a.apply₂ (m.apply₂ &0 &2) (m.apply₂ &1 &2))
+
+end sentences
+
 /-- The language of monoids -/
 protected def monoid : language :=
+language.mk₂ unit empty unit empty empty
+
+/-- The language of additive monoids -/
+protected def add_monoid : language :=
 language.mk₂ unit empty unit empty empty
 
 /-- The language of groups -/
 protected def group : language :=
 language.mk₂ unit unit unit empty empty
 
+/-- The language of additive groups -/
+protected def add_group : language :=
+language.mk₂ unit unit unit empty empty
+
 /-- The language of rings -/
 protected def ring : language :=
-language.sum language.group language.monoid
+language.add_group.sum language.monoid
 
-variable {α : Type u}
+variables (L : language.{u v}) (L' : language.{u' v'})
 
-namespace ring
+/-- A language having a symbol representing `0`. -/
+class has_zero_symb := (symb : L.constants)
 
-/-- The function symbol representing zero. -/
-def zero : language.ring.constants := sum.inl ⟨⟩
+/-- A language having a symbol representing `1`. -/
+class has_one_symb := (symb : L.constants)
 
-/-- The function symbol representing one. -/
-def one : language.ring.constants := sum.inr ⟨⟩
+/-- A language having a symbol representing `-`. -/
+class has_neg_symb := (symb : L.functions 1)
 
-/-- The function symbol representing negation. -/
-def neg : language.ring.functions 1 := sum.inl ⟨⟩
+/-- A language having a symbol representing `⁻¹`. -/
+class has_inv_symb := (symb : L.functions 1)
 
-/-- The function symbol representing addition. -/
-def add : language.ring.functions 2 := sum.inl ⟨⟩
+/-- A language having a symbol representing `+`. -/
+class has_add_symb := (symb : L.functions 2)
 
-/-- The function symbol representing multiplication. -/
-def mul : language.ring.functions 2 := sum.inr ⟨⟩
+/-- A language having a symbol representing `*`. -/
+class has_mul_symb := (symb : L.functions 2)
 
-@[simp] instance : has_zero (language.ring.term α) := ⟨ constants.term zero ⟩
+namespace sum
 
-@[simp] instance : has_one (language.ring.term α) := ⟨ constants.term one ⟩
+variables {L} {L'}
 
-@[simp] instance : has_neg (language.ring.term α) :=
-  ⟨ λ x, func language.ring.neg ![x] ⟩
+instance has_zero_symb_of_left [L.has_zero_symb] : (L.sum L').has_zero_symb :=
+{ symb := sum.inl has_zero_symb.symb }
 
-@[simp] instance : has_add (language.ring.term α) :=
-⟨ λ x y, func language.ring.add ![x, y] ⟩
+instance has_zero_symb_of_right [L'.has_zero_symb] : (L.sum L').has_zero_symb :=
+{ symb := sum.inr has_zero_symb.symb }
 
-@[simp] instance : has_mul (language.ring.term α) :=
-⟨ λ x y, func language.ring.mul ![x, y] ⟩
+instance has_one_symb_of_left [L.has_one_symb] : (L.sum L').has_one_symb :=
+{ symb := sum.inl has_one_symb.symb }
 
-@[simp] instance : has_sub (language.ring.term α) := ⟨ λ x y, x + - y ⟩
+instance has_one_symb_of_right [L'.has_one_symb] : (L.sum L').has_one_symb :=
+{ symb := sum.inr has_one_symb.symb }
 
-instance : has_pow (language.ring.term α) ℕ := ⟨ λ t n, npow_rec n t ⟩
+instance has_neg_symb_of_left [L.has_neg_symb] : (L.sum L').has_neg_symb :=
+{ symb := sum.inl has_neg_symb.symb }
 
-@[simp] lemma pow_zero (t : language.ring.term α) : t ^ 0 = 1 := rfl
-@[simp] lemma pow_succ {n} (t : language.ring.term α) : t ^ (n + 1) = t * t ^ n := rfl
+instance has_neg_symb_of_right [L'.has_neg_symb] : (L.sum L').has_neg_symb :=
+{ symb := sum.inr has_neg_symb.symb }
 
-end ring
+instance has_add_symb_of_left [L.has_add_symb] : (L.sum L').has_add_symb :=
+{ symb := sum.inl has_add_symb.symb }
+
+instance has_add_symb_of_right [L'.has_add_symb] : (L.sum L').has_add_symb :=
+{ symb := sum.inr has_add_symb.symb }
+
+instance has_mul_symb_of_left [L.has_mul_symb] : (L.sum L').has_mul_symb :=
+{ symb := sum.inl has_mul_symb.symb }
+
+instance has_mul_symb_of_right [L'.has_mul_symb] : (L.sum L').has_mul_symb :=
+{ symb := sum.inr has_mul_symb.symb }
+
+end sum
+
+namespace monoid
+
+instance has_one_symb : language.monoid.has_one_symb := { symb := ⟨⟩ }
+
+instance has_mul_symb : language.monoid.has_mul_symb := { symb := ⟨⟩ }
+
+end monoid
+
+namespace add_monoid
+
+instance has_zero_symb : language.add_monoid.has_zero_symb := { symb := ⟨⟩ }
+
+instance add_monoid.has_add_symb : language.add_monoid.has_add_symb := { symb := ⟨⟩ }
+
+end add_monoid
+
+namespace group
+
+instance group.has_one_symb : language.group.has_one_symb := { symb := ⟨⟩ }
+
+instance group.has_inv_symb : language.group.has_inv_symb := { symb := ⟨⟩ }
+
+instance group.has_mul_symb : language.group.has_mul_symb := { symb := ⟨⟩ }
+
+end group
+
+namespace add_group
+
+instance add_group.has_zero_symb : language.add_group.has_zero_symb := { symb := ⟨⟩ }
+
+instance add_group.has_neg_symb : language.add_group.has_neg_symb := { symb := ⟨⟩ }
+
+instance add_group.has_add_symb : language.add_group.has_add_symb := { symb := ⟨⟩ }
+
+end add_group
+
+-- instance why : language.ring.has_one_symb := by apply_instance
+
+variables {L} {α : Type*}
+
+instance [has_zero_symb L] : has_zero (L.term α) := { zero := has_zero_symb.symb.term }
+
+instance [has_one_symb L] : has_one (L.term α) := { one := has_one_symb.symb.term }
+
+instance [has_neg_symb L] : has_neg (L.term α) := { neg := λ x, func has_neg_symb.symb ![x] }
+
+instance [has_inv_symb L] : has_inv (L.term α) := { inv := λ x, func has_inv_symb.symb ![x] }
+
+instance [has_add_symb L] : has_add (L.term α) := { add := λ x y, func has_add_symb.symb ![x, y] }
+
+instance [has_mul_symb L] : has_mul (L.term α) := { mul := λ x y, func has_mul_symb.symb ![x, y] }
+
+section term_pow
+
+variables [has_one_symb L] [has_mul_symb L]
+
+instance : has_pow (L.term α) ℕ := ⟨ λ t n, npow_rec n t ⟩
+
+@[simp] lemma pow_zero (t : L.term α) : t ^ 0 = 1 := rfl
+@[simp] lemma pow_succ {n} (t : L.term α) : t ^ (n + 1) = t * t ^ n := rfl
+
+end term_pow
 
 /-- Any type with instances of `has_one` and `has_mul` is a
   structure in the language of monoids. -/
@@ -84,9 +207,21 @@ def monoid.Structure_of_has_one_has_mul {α : Type*} [has_one α] [has_mul α] :
   language.monoid.Structure α :=
 Structure.mk₂ (λ _, 1) empty.elim (λ _, has_mul.mul) empty.elim empty.elim
 
+/-- Any type with instances of `has_zero` and `has_add` is a
+  structure in the language of additive monoids. -/
+def add_monoid.Structure_of_has_zero_has_add {α : Type*} [has_zero α] [has_add α] :
+  language.monoid.Structure α :=
+Structure.mk₂ (λ _, 0) empty.elim (λ _, has_add.add) empty.elim empty.elim
+
 /-- Any type with instances of `has_one`, `has_inv` and `has_mul` is a
   structure in the language of groups. -/
-def group_Structure_of_has_zero_has_neg_has_add {α : Type} [has_zero α] [has_neg α] [has_add α] :
+def group.Structure_of_has_one_has_inv_has_mul {α : Type} [has_one α] [has_inv α] [has_mul α] :
+  language.group.Structure α :=
+Structure.mk₂ (λ _, 1) (λ _, has_inv.inv) (λ _, has_mul.mul) empty.elim empty.elim
+
+/-- Any type with instances of `has_zero`, `has_neg` and `has_add` is a
+  structure in the language of additive groups. -/
+def add_group.Structure_of_has_zero_has_neg_has_add {α : Type} [has_zero α] [has_neg α] [has_add α] :
   language.group.Structure α :=
 Structure.mk₂ (λ _, 0) (λ _, has_neg.neg) (λ _, has_add.add) empty.elim empty.elim
 
@@ -94,79 +229,88 @@ Structure.mk₂ (λ _, 0) (λ _, has_neg.neg) (λ _, has_add.add) empty.elim emp
 def _root_.monoid.Structure (M : Type) [monoid M] : language.monoid.Structure M :=
 monoid.Structure_of_has_one_has_mul
 
+/-- Any additive monoid is a structure in the language of additive monoids. -/
+def _root_.add_monoid.Structure (M : Type) [add_monoid M] : language.monoid.Structure M :=
+add_monoid.Structure_of_has_zero_has_add
+
 /-- Any group is a structure in the language of groups. -/
+def _root_.group.Structure (G : Type) [group G] : language.group.Structure G :=
+group.Structure_of_has_one_has_inv_has_mul
+
+/-- Any additive group is a structure in the language of additive groups. -/
 def _root_.add_comm_group.Structure (G : Type) [add_comm_group G] : language.group.Structure G :=
-group_Structure_of_has_zero_has_neg_has_add
+add_group.Structure_of_has_zero_has_neg_has_add
 
 /-- Any ring is a structure in the language of ring. -/
 def _root_.ring.Structure (R : Type*) [ring R] : language.ring.Structure R :=
 @language.sum_Structure _ _ _ (add_comm_group.Structure R) (monoid.Structure R)
 
-namespace functions
+section sentences
 
-variables {L : language} (c₀ c₁ : L.constants) (i : L.functions 1) (a : L.functions 2)
-  (m : L.functions 2)
+/-- The sentence indicating associativity of addition -/
+protected def add_assoc [has_add_symb L] : L.sentence := language.assoc has_add_symb.symb
 
-/-- The sentence indicating that a binary function symbol is commutative. -/
-protected def comm : L.sentence := ∀' ∀' (m.apply₂ &0 &1 =' m.apply₂ &1 &0)
+/-- The sentence indicating commutativity of addition -/
+protected def add_comm [has_add_symb L] : L.sentence := language.comm has_add_symb.symb
 
-/-- The sentence indicating that a binary function symbol is associative. -/
-protected def assoc : L.sentence :=
-∀' ∀' ∀' (m.apply₂ (m.apply₂ &0 &1) &2 =' m.apply₂ &0 (m.apply₂ &1 &2))
+/-- The sentence indicating associativity of multiplication -/
+protected def mul_assoc [has_mul_symb L] : L.sentence := language.assoc has_mul_symb.symb
 
-/-- The sentence indicating that applying a constant symbol on the right of
-  a binary symbol is the identity. -/
-protected def mul_id : L.sentence :=
-∀' (m.apply₂ &0 c₁.term =' &0)
+/-- The sentence indicating commutativity of multiplication -/
+protected def mul_comm [has_mul_symb L] : L.sentence := language.comm has_mul_symb.symb
 
-/-- The sentence indicating that applying a constant symbol on the right of
-  a binary symbol is the identity. -/
-protected def id_mul : L.sentence :=
-∀' (m.apply₂ c₁.term &0 =' &0)
+/-- The sentence indicating that zero is a right identity to addition -/
+protected def add_zero [has_zero_symb L] [has_add_symb L] : L.sentence :=
+id_right has_zero_symb.symb has_add_symb.symb
 
-/-- The sentence indicating that left composing a unary symbol with a binary symbol
-  is equal to a constant symbol. -/
-protected def inv_mul : L.sentence :=
-∀' (m.apply₂ (i.apply₁ &0) &0 =' c₁.term)
+/-- The sentence indicating that zero is a left identity to addition -/
+protected def zero_add [has_zero_symb L] [has_add_symb L] : L.sentence :=
+id_left has_zero_symb.symb has_add_symb.symb
 
-/-- The sentence indicating that left composing a unary symbol with a binary symbol
-  is equal to a constant symbol. -/
-protected def mul_inv : L.sentence :=
-∀' (m.apply₂ &0 (i.apply₁ &0) =' c₁.term)
+/-- The sentence indicating that one is a right identity to addition -/
+protected def mul_one [has_one_symb L] [has_mul_symb L] : L.sentence :=
+id_right has_one_symb.symb has_mul_symb.symb
 
-/-- The sentence indicating that a binary function symbol distributes over another -/
-protected def add_mul : L.sentence :=
-∀' ∀' ∀' (m.apply₂ (a.apply₂ &0 &1) &2 =' a.apply₂ (m.apply₂ &0 &2) (m.apply₂ &1 &2))
+/-- The sentence indicating that one is a left identity to addition -/
+protected def one_mul [has_one_symb L] [has_mul_symb L] : L.sentence :=
+id_left has_one_symb.symb has_mul_symb.symb
 
-/-- The sentence indicating that multiplication has an inverse away from a constant zero -/
-protected def field_inv : L.sentence :=
-∀' (&0 =' c₀.term ⊔ ∃' (m.apply₂ &1 &0 =' c₁.term))
+/-- The sentence indicating that negation is the left inverse to addition -/
+protected def neg_add_self [has_zero_symb L] [has_neg_symb L] [has_add_symb L] : L.sentence :=
+cancel_left has_zero_symb.symb has_neg_symb.symb has_add_symb.symb
 
-end functions
+/-- The sentence indicating that negation is the right inverse to addition -/
+protected def add_neg_self [has_zero_symb L] [has_neg_symb L] [has_add_symb L] : L.sentence :=
+cancel_right has_zero_symb.symb has_neg_symb.symb has_add_symb.symb
 
-section ring_theories
+/-- The sentence indicating that left multiplication distributes over addition -/
+protected def mul_add [has_add_symb L] [has_mul_symb L] : L.sentence :=
+language.distrib has_add_symb.symb has_mul_symb.symb
 
-open language.ring
+end sentences
+
+instance ring.has_zero_symb : language.ring.has_zero_symb := sum.has_zero_symb_of_left
+instance ring.has_one_symb : language.ring.has_one_symb := sum.has_one_symb_of_right
+instance ring.has_neg_symb : language.ring.has_neg_symb := sum.has_neg_symb_of_left
+instance ring.has_add_symb : language.ring.has_add_symb := sum.has_add_symb_of_left
+instance ring.has_mul_symb : language.ring.has_mul_symb := sum.has_mul_symb_of_right
 
 /-- The theory of commutative rings. -/
 def Theory.comm_ring : Theory language.ring :=
-{ functions.assoc add,
-  functions.mul_id zero add,
-  functions.comm add,
-  functions.inv_mul zero neg add,
-  functions.assoc mul,
-  functions.mul_id one mul,
-  functions.comm mul,
-  functions.add_mul add mul }
+{ language.add_assoc,
+  language.add_zero,
+  language.add_comm,
+  language.neg_add_self,
+  language.mul_assoc,
+  language.mul_one,
+  language.mul_comm,
+  language.mul_add }
 
 /-- The theory of fields. -/
 def Theory.field : Theory language.ring :=
 Theory.comm_ring ∪ {
-  functions.field_inv zero one mul,
+  ∀' (&0 =' 0 ⊔ ∃' ((&1 * &0) =' 1)),
   sentence.card_ge _ 1 }
-
-end ring_theories
 
 end language
 end first_order
-
